Finished a couple proofs and left some admits in others.

graph_inst.v
@@ -65,17 +65,39 @@ Module Bleh : Graphs PositiveOrderedTypeBits.
       if (mset.mem x1 (vertices g) && mset.mem x2 (vertices g))
       then Node x1 ([x2]) g
       else g.
-  
-  Parameter remove_vertex : t -> node -> t.
-  Parameter remove_edge : t -> node * node -> t.
+  Fixpoint remove_vertex (g : graph) (n : node) :=
+  match g with
+  |Empty => Empty
+  |Node n' adj g' => if Pos.eqb n' n then remove_vertex g' n
+       else  Node n' (mset.remove n adj) (remove_vertex g' n)
+  end.
 
+(*It is possible to make a graph with edges form a-b and b-a but since it is undirected maybe that should not be allowed or should be forced, need to come back to it*)
+    
+Fixpoint remove_edge (g : graph) (e : (node * node) ) :=
+  let x := (fst e) in
+  let y := (snd e) in
+  match g with
+  |Empty => Empty
+  |Node n adj g' => if Pos.eqb n x then Node n (mset.remove y adj) g'
+                   else Node n adj (remove_edge g' e)
+  end.
+
+
+Fixpoint neighborhood (g : graph) (x : node) : node_set:=
+  match g with
+  | Empty => mset.empty
+  | Node y adj g' =>
+    if Pos.eqb x y then  mset.union adj (neighborhood g' x)
+    else if mset.mem x adj then mset.add y (neighborhood g' x)
+         else neighborhood g' x
+  end.
   
-  
+    
   Definition is_vertex : t -> node -> bool :=
     fun g x => mset.mem x (vertices g).
   Definition is_edge : t -> node * node -> bool :=
     fun g x => msetPair.mem x (edges g).
-  Parameter neighborhood : t -> node -> node_set.
   Lemma empty_vertices : vertices empty = mset.empty.
   Proof. reflexivity. Qed.
   Lemma empty_edges : edges empty = msetPair.empty.
@@ -98,7 +120,11 @@ Module Bleh : Graphs PositiveOrderedTypeBits.
       simpl. rewrite mset.fold_spec.
       simpl. apply msetPair.add_spec.
       auto.
-Qed.
+    Qed.
+
+    (* Lemma notin_vert_eq : *)
+    (*   forall ( *)
+   
   Lemma add_edges :
     forall (e : node * node) (g : t),
       mset.In (fst e) (vertices g) ->
@@ -110,7 +136,7 @@ Qed.
     inversion H.
     apply mset.mem_spec in H; apply mset.mem_spec in H0.
     case_eq (mset.mem n (mset.add n1 (vertices g)));
-    case_eq (mset.mem n0 (mset.add n1 (vertices g))).
+      case_eq (mset.mem n0 (mset.add n1 (vertices g))).
     simpl (_ && _); cbv iota.
     {
       intros H1 H2.
@@ -120,11 +146,21 @@ Qed.
     }
     {
       intros H1 H2.
-      simpl (_ && _); cbv iota. 
+      simpl (_ && _); cbv iota.
       
-(* given H and H0 since n and n0 are not in v (g) then they must be equal to n1 and n2 then it should be possible to say that given Node n1 n2 being visible that (n, n0) is in the graph.*)
-      Admitted.
-
+      admit.
+    }
+    {
+      intros.
+      simpl ( _ && _); cbv iota.
+      admit.
+    }
+    {
+      intros H1 H2.
+      simpl (_ && _); cbv iota.
+      admit.
+   }
+Admitted.
 
     Lemma add_vertices_other :
       forall (x y : node) (g : t),
@@ -132,40 +168,175 @@ Qed.
     Proof.
       split; intros; induction g.
       inversion H0.
-    Admitted.
-    Parameter add_edges_other :
+      {
+       unfold add_vertex.
+       simpl. apply mset.add_spec.
+       auto.
+      }
+      {
+       simpl.
+       inversion H0.
+       symmetry in H2;
+       contradiction.
+       auto. auto.
+      }
+
+       simpl. apply mset.add_spec.
+       unfold add_vertex in H0.
+       simpl in H0. apply mset.add_spec in H0.
+       destruct H0.
+       symmetry in H0.
+       contradiction.
+       apply mset.add_spec in H0.
+       auto.
+    Qed.
+
+    Lemma add_edges_other :
       forall (e1 e2 : node * node) (g : t),
-        e1 <> e2 -> In e2 (edges g) <-> In e2 (edges (add_edge g e1)).
-    Parameter add_vertices_pres_edges :
-      forall (x : node) (g : t), Equal (edges (add_vertex g x)) (edges g).
-    Parameter add_edges_pres_vertices :
+        e1 <> e2 -> msetPair.In e2 (edges g) <-> msetPair.In e2 (edges (add_edge g e1)).
+    Proof.
+      intros; split; induction g; auto.
+      {
+       inversion 1.
+      }
+      {
+        intros. unfold add_edge. 
+        simpl.  destruct e1.
+        
+        case_eq (mset.mem n1 (mset.add n (vertices g)));
+          case_eq ( mset.mem n2 (mset.add n (vertices g))).
+       
+          intros H1 H2; simpl (_ && _); cbv iota.
+          apply msetPair.add_spec;
+          auto.
+          auto.
+          auto. auto.
+      }
+      {
+        intros.
+        unfold add_edge in H0.
+        simpl (_ && _) in H0. cbv iota in H0.
+        simpl ((let (_,_) := e1 in Empty)) in H0.
+        admit.
+      }
+      {
+        intros.
+        admit.
+      }
+    Admitted.
+       
+       
+
+
+
+
+    Lemma add_vertices_pres_edges :
+      forall (x : node) (g : t), msetPair.Equal (edges (add_vertex g x)) (edges g).
+    Proof.
+      intros.
+      unfold add_vertex.
+      cbv.
+      auto.
+      (* This was pretty funny.  Given that is takes so long to compute it's probably worth comming back and doing this a better way.*)
+    Qed.
+    
+    Lemma add_edges_pres_vertices :
       forall (x : node * node) (g : t),
-        Equal (vertices (add_edge g x)) (vertices g).
-    Parameter remove_vertices :
-      forall (x : node) (g : t), ~ In x (vertices (remove_vertex g x)).
-    Parameter remove_edges :
-      forall (e : node * node) (g : t), ~ In e (edges (remove_edge g e)).
-     Parameter remove_vertices_edges_l :
-       forall (x1 : node) (g : t) (x2 : node),
-       ~ In (x1, x2) (edges (remove_vertex g x1)).
-     Parameter remove_vertices_edges_r :
-       forall (x1 : node) (g : t) (x2 : node),
-       ~ In (x2, x1) (edges (remove_vertex g x1)).
-     Parameter remove_vertices_other :
-       forall (x y : node) (g : t),
-       x <> y -> In y (vertices g) <-> In y (vertices (remove_vertex g x)).
-     Parameter remove_edges_other :
-       forall (e1 e2 : node * node) (g : t),
-       e1 <> e2 -> In e2 (edges g) <-> In e2 (edges (remove_edge g e1)).
-     Parameter is_vertex_vertices :
-       forall (x : elt) (g : t), In x (vertices g) <-> is_vertex g x = true.
-     Parameter is_edge_edges :
-       forall (e : elt) (g : t), In e (edges g) <-> is_edge g e = true.
-     Parameter neighborhood_prop :
-       forall (x : node) (y : elt) (g : t),
-       In y (neighborhood g x) <-> In (x, y) (edges g).
-     Parameter edges_proper_l :
-       forall (x : elt) (g : t), In x (edges g) -> In (fst x) (vertices g).
-     Parameter edges_proper_r :
-       forall (x : elt) (g : t), In x (edges g) -> In (snd x) (vertices g).
-Print Graphs.
+        mset.Equal (vertices (add_edge g x)) (vertices g).
+    Proof.
+      intros.
+      unfold add_edge. destruct x.
+      case_eq (mset.mem n (vertices g));
+        case_eq ( mset.mem n0 (vertices g)).
+      {
+        intros H1 H2; simpl (_ && _); cbv iota.
+        simpl. 
+        admit.
+      }
+      {
+        intros H1 H2; simpl (_ && _); cbv iota.
+        reflexivity.
+      }
+      {
+        intros H1 H2; simpl (_ && _); cbv iota.
+        reflexivity.
+      }
+      intros H1 H2; simpl (_ && _); cbv iota.
+      reflexivity.
+    Admitted.
+    
+
+    Lemma remove_vertices :
+      forall (x : node) (g : t), ~ mset.In x (vertices (remove_vertex g x)).
+    Proof.
+      intros.
+      induction g.
+      simpl. unfold not. intros. apply mset.mem_spec in H.
+      inversion H.
+      unfold not.
+      intros. apply mset.mem_spec in H. 
+      simpl in H.
+    Admitted.
+
+    Lemma remove_edges :
+      forall (e : node * node) (g : t), ~ msetPair.In e (edges (remove_edge g e)).
+    Proof.
+      intros.
+      unfold not. intros.
+      Admitted.
+
+
+    Lemma remove_vertices_edges_l :
+        forall (x1 : node) (g : t) (x2 : node),
+          ~ msetPair.In (x1, x2) (edges (remove_vertex g x1)).
+    Proof.
+      intros. unfold not. intros.
+      induction g.
+      simpl in H. inversion H.
+    Admitted.
+    
+    
+      
+    Lemma remove_vertices_edges_r :
+        forall (x1 : node) (g : t) (x2 : node),
+          ~ msetPair.In (x2, x1) (edges (remove_vertex g x1)).
+    Proof.
+      intros.
+    Admitted.
+    
+
+
+    Lemma remove_vertices_other :
+        forall (x y : node) (g : t),
+          x <> y ->  mset.In y (vertices g) <-> mset.In y (vertices (remove_vertex g x)).
+    Proof.
+      intros.
+      split. intros.
+      induction g.
+      auto. simpl.
+      destruct (n =? x)%positive.
+      Focus 2.
+      simpl.
+      apply mset.add_spec.
+      apply mset.add_spec in H0.
+      destruct H0.
+      auto.
+      auto.
+      admit.
+    Admitted.
+    
+Parameter remove_edges_other :
+        forall (e1 e2 : node * node) (g : t),
+          e1 <> e2 -> In e2 (edges g) <-> In e2 (edges (remove_edge g e1)).
+      Parameter is_vertex_vertices :
+        forall (x : elt) (g : t), In x (vertices g) <-> is_vertex g x = true.
+      Parameter is_edge_edges :
+        forall (e : elt) (g : t), In e (edges g) <-> is_edge g e = true.
+      Parameter neighborhood_prop :
+        forall (x : node) (y : elt) (g : t),
+          In y (neighborhood g x) <-> In (x, y) (edges g).
+      Parameter edges_proper_l :
+        forall (x : elt) (g : t), In x (edges g) -> In (fst x) (vertices g).
+      Parameter edges_proper_r :
+        forall (x : elt) (g : t), In x (edges g) -> In (snd x) (vertices g).
+      Print Graphs.
